more general construction

theories/util.v
@@ -1,20 +1,37 @@
 From iris Require Import bi.bi.
 From bedrock Require Import IrisBridge.
 Import ChargeNotation.
+Open Scope N_scope.
 Section lift.
   Context {PROP: bi}.
   Notation paddr := N.
   Variable byte_at : forall (hpa:paddr) (hpaFrac : Qp) (value : N), PROP.
 
-  Definition short_at (pa : paddr) (q:Qp) (v : N) : PROP :=
-    byte_at pa q (N.land v (2^8 - 1)) **
-            byte_at (pa + 1)%N q (N.shiftr v 8).
+  Fixpoint lift n (pa : paddr) (q:Qp) (v : N) :=
+    match n with
+    | O => byte_at pa q v
+    | S n => let bytesize :N := (2^(N.of_nat n)) in
+            let bitsize := (8*bytesize)%N in
+            lift n pa q (N.land v (2^bitsize - 1))
+            ** lift n (pa+bytesize) q (N.shiftr v bitsize)
+    end.
 
-  Definition word_at (pa : paddr) (q : Qp) (v : N) : PROP :=
-    short_at pa q (N.land v (2^16 - 1))**
-             short_at (pa + 2)%N q (N.shiftr v 16).
+  Section test.
 
-  Definition dword_at (pa : paddr) (q : Qp) (v : N) : PROP :=
-    word_at pa q (N.land v (2^32 - 1))**
-            word_at (pa + 4)%N q (N.shiftr v 32).
+    Local Definition short_at (pa : paddr) (q:Qp) (v : N) : PROP :=
+      byte_at pa q (N.land v (2^8 - 1))%N **
+              byte_at (pa + 1)%N q (N.shiftr v 8).
+
+    Local Definition word_at (pa : paddr) (q : Qp) (v : N) : PROP :=
+      short_at pa q (N.land v (2^16 - 1))**
+               short_at (pa + 2)%N q (N.shiftr v 16).
+
+    Example t1 pa q v : short_at pa q v = lift 1 pa q v.
+    reflexivity.
+    Qed.
+    Example t2 pa q v : word_at pa q v = lift 2 pa q v.
+    reflexivity.
+    Qed.
+  End test.
+
 End lift.
